maybe dd double recursion backwards will try flipping

theories/Logic/inverse_ug_l.v
@@ -12,27 +12,31 @@ Require Import List.
 Require Import Lia.
 Import ListNotations.
 
-Definition ug_left_inv_formula (phi A : formula) (b : bool) : formula := formula_sub phi (univ A) A 0 b.
+Definition ug_left_inv_formula (phi A : formula) (b : bool) : formula := formula_sub phi (univ A) A b.
 
 Lemma ug_l_inv_form_depth_le :
     forall (phi A : formula) (b : bool),
-        form_depth (formula_sub phi (univ A) A 0 b) <= form_depth phi.
+        form_depth (formula_sub phi (univ A) A b) <= form_depth phi.
 Proof.
 intros phi A b.
 unfold formula_sub.
-case form_equiv eqn:EQF.
+case form_eqb eqn:EQF.
 destruct b.
-rewrite (form_equiv_preserves_depth _ _ _ EQF).
+apply form_eqb_eq in EQF.
+subst.
 unfold form_depth;
 fold form_depth.
 all : lia.
 Qed.
 
-Definition ug_left_inv_batch (gamma : list formula) (A : formula) (d : nat) (S : subst_ind) : list formula := batch_sub gamma (univ A) A d S.
+Definition ug_left_inv_batch (gamma : list formula) (A : formula) (S : subst_ind) : list formula := batch_sub gamma (univ A) A S.
 
 Fixpoint ptree_ug_l_inv_fit
-  (P : ptree) (A : formula) (S : subst_ind) : ptree :=
-let REC := (fun PT SI => (ptree_ug_l_inv_fit PT A SI)) in
+  (P : ptree) (A : formula) (S : subst_ind) (depth : nat) : ptree :=
+match depth with
+| 0 => P
+| S d =>
+let REC := (fun PT SI DEP => (ptree_ug_l_inv_fit PT A SI DEP)) in
 match P, S with
 | bot, _ => P
 
@@ -40,53 +44,54 @@ match P, S with
 
 | equal v1 v2, _ => P
 
-| loop_head OC gamma delta alpha P_Target, _ => loop_head OC (ug_left_inv_batch gamma A 0 S) delta alpha (REC P_Target S)
+| loop_head OC gamma delta alpha P_Target, _ => loop_head OC (ug_left_inv_batch gamma A S) delta alpha (REC P_Target S d)
 
-| @sub_l OC gamma delta phi v1 v2 alpha P', s1 :: s2 :: S' => @sub_l OC (ug_left_inv_batch gamma A 0 S') delta (formula_sub (shift_substitution phi v1 v2) (univ A) A v2 s2) v1 v2 alpha (REC P' (s1 :: s2 :: S'))
+| @sub_l OC gamma delta phi v1 v2 alpha P', s1 :: s2 :: S' => @sub_l OC (ug_left_inv_batch gamma A S') delta (ug_left_inv_formula phi A s2) v1 v2 alpha (REC (ptree_ug_l_inv_fit P' (shift_substitution A (Datatypes.S v1) v2) (false :: s2 :: repeat false (length S')) d) (s1 :: false :: S') d)
 
-| @sub_r OC gamma delta phi v1 v2 alpha P', s :: S' => @sub_r OC (ug_left_inv_batch gamma A 0 S') delta phi v1 v2 alpha (REC P' (s :: S'))
+| @sub_r OC gamma delta phi v1 v2 alpha P', s :: S' => @sub_r OC (ug_left_inv_batch gamma A S') delta phi v1 v2 alpha (REC P' (s :: S') d)
 
-| @con_l OC gamma delta phi alpha P', s :: S' => @con_l OC (ug_left_inv_batch gamma A 0 S') delta (ug_left_inv_formula phi A s) alpha (REC P' (s :: s :: S'))
+| @con_l OC gamma delta phi alpha P', s :: S' => @con_l OC (ug_left_inv_batch gamma A S') delta (ug_left_inv_formula phi A s) alpha (REC P' (s :: s :: S') d)
 
-| @con_r OC gamma delta phi alpha P', _ => @con_r OC (ptree_left (REC P' S)) delta phi alpha (REC P' S)
+| @con_r OC gamma delta phi alpha P', _ => @con_r OC (ptree_left (REC P' S d)) delta phi alpha (REC P' S d)
 
-| @refl OC gamma delta v alpha P', _ => @refl OC (ug_left_inv_batch gamma A 0 S) delta v alpha (ptree_ug_l_inv_fit P' A (false :: S))
-
-
-| @ex_l OC gamma delta n alpha P', _ => @ex_l OC (ptree_left (REC P' (unbury S n))) delta n alpha (REC P' (unbury S n))
-
-| @ex_r OC gamma delta n alpha P', _ => @ex_r OC (ptree_left (REC P' S)) delta n alpha (REC P' S)
+| @refl OC gamma delta v alpha P', _ => @refl OC (ug_left_inv_batch gamma A S) delta v alpha (ptree_ug_l_inv_fit P' A (false :: S) d)
 
 
-| @wkn_l OC gamma delta phi alpha P', s :: S' => @wkn_l OC (ug_left_inv_batch gamma A 0 S') delta (ug_left_inv_formula phi A s) alpha (REC P' S')
+| @ex_l OC gamma delta n alpha P', _ => @ex_l OC (ptree_left (REC P' (unbury S n) d)) delta n alpha (REC P' (unbury S n) d)
 
-| @wkn_r OC gamma delta phi alpha P', _ => @wkn_r OC (ptree_left (REC P' S)) delta phi alpha (REC P' S)
+| @ex_r OC gamma delta n alpha P', _ => @ex_r OC (ptree_left (REC P' S d)) delta n alpha (REC P' S d)
 
-| @rst OC gamma delta kappa alpha P', _ => @rst OC (ptree_left (REC P' S)) delta kappa alpha (REC P' S)
+
+| @wkn_l OC gamma delta phi alpha P', s :: S' => @wkn_l OC (ug_left_inv_batch gamma A S') delta (ug_left_inv_formula phi A s) alpha (REC P' S' d)
+
+| @wkn_r OC gamma delta phi alpha P', _ => @wkn_r OC (ptree_left (REC P' S d)) delta phi alpha (REC P' S d)
+
+| @rst OC gamma delta kappa alpha P', _ => @rst OC (ptree_left (REC P' S d)) delta kappa alpha (REC P' S d)
 
 | @ug_l OC gamma delta phi alpha P', s :: S' => match form_eqb phi A, s with
-    | true, true => REC P' (false :: S')
-    | _, _ => let SI := (false :: S') in @ug_l OC (ug_left_inv_batch gamma A 0 S') delta phi alpha (REC P' SI)
+    | true, true => REC P' (false :: S') d
+    | _, _ => let SI := (false :: S') in @ug_l OC (ug_left_inv_batch gamma A S') delta phi alpha (REC P' SI d)
     end
 
-| @ug_r OC gamma delta phi alpha P', _ => @ug_r OC (ptree_left (REC P' S)) delta phi alpha (REC P' S)
+| @ug_r OC gamma delta phi alpha P', _ => @ug_r OC (ptree_left (REC P' S d)) delta phi alpha (REC P' S d)
 
-| @bnd_l OC gamma delta phi lambda kappa alpha P', s :: S' => @bnd_l OC (ug_left_inv_batch gamma A 0 S') delta phi lambda kappa alpha (REC P' (false :: S'))
+| @bnd_l OC gamma delta phi lambda kappa alpha P', s :: S' => @bnd_l OC (ug_left_inv_batch gamma A S') delta phi lambda kappa alpha (REC P' (false :: S') d)
 
-| @bnd_r OC gamma delta phi lambda kappa alpha P', _ => @bnd_r OC (ptree_left (REC P' S)) delta phi lambda kappa alpha (REC P' S)
+| @bnd_r OC gamma delta phi lambda kappa alpha P', _ => @bnd_r OC (ptree_left (REC P' S d)) delta phi lambda kappa alpha (REC P' S d)
 
-| @imp_l OC gamma delta phi psi alpha1 alpha2 P1 P2, s :: S' =>  @imp_l OC (ug_left_inv_batch gamma A 0 S') delta phi psi alpha1 alpha2 (REC P1 (false :: S')) (REC P2 S')
+| @imp_l OC gamma delta phi psi alpha1 alpha2 P1 P2, s :: S' =>  @imp_l OC (ug_left_inv_batch gamma A S') delta phi psi alpha1 alpha2 (REC P1 (false :: S') d) (REC P2 S' d)
 
-| @imp_r OC gamma delta phi psi alpha P', _ => @imp_r OC (ug_left_inv_batch gamma A 0 S) delta phi psi alpha (REC P' (false :: S))
+| @imp_r OC gamma delta phi psi alpha P', _ => @imp_r OC (ug_left_inv_batch gamma A S) delta phi psi alpha (REC P' (false :: S) d)
 
-| @cut OC gamma delta phi alpha1 alpha2 P1 P2, _ => @cut OC (ug_left_inv_batch gamma A 0 S) delta phi alpha1 alpha2 (REC P1 S) (REC P2 (false :: S))
+| @cut OC gamma delta phi alpha1 alpha2 P1 P2, _ => @cut OC (ug_left_inv_batch gamma A S) delta phi alpha1 alpha2 (REC P1 S d) (REC P2 (false :: S) d)
 
 | _ , _ => P
+end
 end.
 
 Definition ptree_ug_l_inv (P : ptree) (A : formula) (S : subst_ind) : ptree :=
 match nat_eqb (length (ptree_left P)) (length S) with
-| true => ptree_ug_l_inv_fit P A S
+| true => ptree_ug_l_inv_fit P A S (ptree_height P)
 | false => P
 end.
 
@@ -94,7 +99,7 @@ Lemma ptree_ug_l_inv_fit_true :
     forall {P : ptree} {A : formula},
         forall {S : subst_ind},
             nat_eqb (length (ptree_left P)) (length S) = true ->
-                (ptree_ug_l_inv_fit P A S) = (ptree_ug_l_inv P A S).
+                (ptree_ug_l_inv_fit P A S (ptree_height P)) = (ptree_ug_l_inv P A S).
 Proof. intros P A S EQ. unfold ptree_ug_l_inv. rewrite EQ. reflexivity. Qed.
 
 Lemma ptree_ug_l_inv_left :
@@ -102,7 +107,7 @@ Lemma ptree_ug_l_inv_left :
         struct_valid P ->
             forall (S : subst_ind),
                 ptree_left (ptree_ug_l_inv P A S) =
-                    (ug_left_inv_batch (ptree_left P) A 0 S).
+                    (ug_left_inv_batch (ptree_left P) A S).
 Proof.
 intros P A.
 induction P;
@@ -111,6 +116,8 @@ unfold ptree_ug_l_inv;
 unfold ug_left_inv_batch, batch_sub;
 case nat_eqb eqn:EQ;
 try reflexivity;
+unfold ptree_height;
+fold ptree_height;
 unfold ptree_ug_l_inv_fit;
 fold ptree_ug_l_inv_fit;
 unfold ptree_left in EQ;
@@ -149,10 +156,10 @@ all : try rewrite (batch_sub_fit_true EQ);
       unfold form_equiv, ug_left_inv_formula, ug_left_inv_batch.
       rewrite batch_sub_fit_true.
       2 : apply EQ.
-      admit. }
+      reflexivity. }
 
 3 : { unfold ptree_left at 1.
-      fold (ptree_left (ptree_ug_l_inv_fit P A (unbury S n))).
+      fold (ptree_left (ptree_ug_l_inv_fit P A (unbury S n) (ptree_height P))).
       rewrite ptree_ug_l_inv_fit_true, <- batch_bury_comm, (IHP PSV).
       reflexivity.
       rewrite bury_length, <- (@bury_unbury _ S n), bury_length in EQ.
@@ -161,8 +168,8 @@ all : try rewrite (batch_sub_fit_true EQ);
 all : destruct S as [ | b S];
       inversion EQ.
 
-4 : unfold formula_sub, form_equiv;
-    fold form_equiv;
+4 : unfold formula_sub, form_eqb;
+    fold form_eqb;
     try rewrite form_equiv_0_eq;
     case (form_eqb phi A) eqn:EQF.
 4 : destruct b.
@@ -188,7 +195,7 @@ all : try unfold ptree_left at 1 2;
     reflexivity.
     rewrite PG.
     apply EQ.
-Admitted.
+Qed.
 
 Lemma ptree_ug_l_inv_right :
     forall (P : ptree) (A : formula),
@@ -217,6 +224,8 @@ unfold ug_left_inv_batch, batch_sub.
 all : subst; 
       case nat_eqb eqn:EQ;
       try reflexivity;
+      unfold ptree_height;
+      fold ptree_height;
       unfold ptree_ug_l_inv_fit;
       fold ptree_ug_l_inv_fit;
       unfold ptree_left in EQ;
@@ -265,6 +274,8 @@ unfold ug_left_inv_batch, batch_sub.
 all : subst; 
       case nat_eqb eqn:EQ;
       try reflexivity;
+      unfold ptree_height;
+      fold ptree_height;
       unfold ptree_ug_l_inv_fit;
       fold ptree_ug_l_inv_fit;
       unfold ptree_left in EQ;
@@ -314,6 +325,8 @@ unfold ug_left_inv_batch, batch_sub.
 all : subst; 
       case nat_eqb eqn:EQ;
       try reflexivity;
+      unfold ptree_height;
+      fold ptree_height;
       unfold ptree_ug_l_inv_fit;
       fold ptree_ug_l_inv_fit;
       unfold ptree_left in EQ;
@@ -343,15 +356,16 @@ Lemma ug_l_formula_inv_vars :
 Proof.
 intros phi A b.
 unfold ug_left_inv_formula, formula_sub.
-case form_equiv eqn:EQF.
+case form_eqb eqn:EQF.
 destruct b.
-rewrite (form_equiv_preserves_ovars _ _ _ EQF).
+apply form_eqb_eq in EQF.
+subst.
 all : reflexivity.
 Qed.
 
 Lemma ptree_ug_l_inv_vars :
     forall (gamma : list formula) (A : formula) (S : subst_ind),
-        flat_map vars_in (ug_left_inv_batch gamma A 0 S) =
+        flat_map vars_in (ug_left_inv_batch gamma A S) =
             flat_map vars_in gamma.
 Proof.
 induction gamma;
@@ -366,7 +380,7 @@ case nat_eqb eqn:EQN.
 unfold flat_map;
 fold (flat_map vars_in).
 rewrite (batch_sub_fit_true EQN).
-fold (ug_left_inv_batch gamma A 0 S).
+fold (ug_left_inv_batch gamma A S).
 rewrite IHgamma.
 fold (ug_left_inv_formula a A b).
 rewrite ug_l_formula_inv_vars.
@@ -463,19 +477,124 @@ all : subst;
 Qed.
 *)
 
-Lemma ptree_ug_l_inv_struct :
-    forall (P : ptree) (A : formula),
-        struct_valid P ->
+
+Lemma ptree_ug_l_inv_height_aux :
+    forall (n : nat) (P : ptree) (A : formula),
+        ptree_height P <= n ->
             forall (S : subst_ind),
-                struct_valid (ptree_ug_l_inv P A S).
+                ptree_height (ptree_ug_l_inv_fit P A S n) <= n.
 Proof.
-intros P.
-induction P;
-try intros AF PSV S;
+induction n;
+intros P A LT S.
+destruct P;
+inversion LT.
+destruct P;
+apply le_S_n in LT;
+unfold ptree_ug_l_inv_fit;
+fold ptree_ug_l_inv_fit;
+unfold ptree_height;
+fold ptree_height.
+
+5,6,7,12,15,17,19 : destruct S as [ | b S].
+
+6 : destruct S as [ | b1 [ | B2 S]].
+
+16 : case (form_eqb phi A) eqn:EQF.
+16 : destruct b.
+
+all : unfold ptree_height in *;
+      fold ptree_height in *;
+      try apply le_n_S;
+      try rewrite EQL';
+      try apply (IHn _ _ LT);
+      try lia.
+
+- apply (IHn _ _ (IHn _ _ LT _) _).
+
+- apply (IHn _ _ (IHn _ _ LT _) _).
+
+- apply le_S, IHn, LT.
+
+- assert ((ptree_height P1) <= n /\ (ptree_height P2) <= n) as [LT1 LT2]. split; lia.
+  pose proof (IHn _ A LT1 (false :: S)) as LT3.
+  pose proof (IHn _ A LT2 S) as LT4.
+  lia.
+
+- assert ((ptree_height P1) <= n /\ (ptree_height P2) <= n) as [LT1 LT2]. split; lia.
+  pose proof (IHn _ A LT1 S) as LT3.
+  pose proof (IHn _ A LT2 (false :: S)) as LT4.
+  lia.
+Qed.
+
+Lemma ptree_ug_l_inv_height :
+    forall (P : ptree) (A : formula) (S : subst_ind),
+        ptree_height (ptree_ug_l_inv_fit P A S (ptree_height P)) <= (ptree_height P).
+Proof. intros P A S. apply (ptree_ug_l_inv_height_aux _ _ _ (le_n _)). Qed.
+
+
+Lemma ptree_ug_l_inv_fit_extra :
+    forall (d1 d2 : nat) (P : ptree) (A : formula) (S : subst_ind),
+        (ptree_height P) <= d1 ->
+            (ptree_height P) <= d2 ->
+                ptree_ug_l_inv_fit P A S d1 = ptree_ug_l_inv_fit P A S d2.
+Proof.
+induction d1;
+intros d2 P A S LT1 LT2.
+destruct P;
+inversion LT1.
+destruct d2.
+destruct P;
+inversion LT2.
+destruct P;
+apply le_S_n in LT1;
+apply le_S_n in LT2;
+unfold ptree_height in *;
+fold ptree_height in *;
+unfold ptree_ug_l_inv_fit;
+fold ptree_ug_l_inv_fit.
+
+6,7,12,15,17,19 : destruct S as [ | b S].
+
+5 : destruct S as [ | b1 [ | b2 S]].
+
+15 : case (form_eqb phi A) eqn:EQF.
+15 : destruct b.
+
+21,31 : assert (ptree_height P1 <= d1 /\ ptree_height P2 <= d1 /\ (ptree_height P1) <= d2 /\ (ptree_height P2) <= d2) as [LT3 [LT4 [LT5 LT6]]]; repeat split; try lia.
+
+all : try rewrite (IHd1 _ _ _ _ LT1 LT2);
+      try rewrite (IHd1 _ _ _ _ LT3 LT5);
+      try rewrite (IHd1 _ _ _ _ LT4 LT6);
+      try rewrite (IHd1 _ _ _ _ LT3);
+      try rewrite (IHd1 _ _ _ _ LT4);
+      try reflexivity.
+
+1 : pose proof (ptree_ug_l_inv_height P (shift_substitution A (Datatypes.S v1) v2) (false :: b2 :: (repeat false (@length bool S)))) as LT3.
+    rewrite <- (IHd1 _ _ _ _ LT1 (le_n _)) in LT3.
+    rewrite (IHd1 _ _ _ _ LT1 LT2) in LT3.
+    rewrite (IHd1 _ _ _ _ (PeanoNat.Nat.le_trans _ _ _ LT3 LT1) (PeanoNat.Nat.le_trans _ _ _ LT3 LT2)).
+    reflexivity.
+Qed.
+
+Lemma ptree_ug_l_inv_struct_aux :
+    forall (d : nat) (P : ptree) (A : formula),
+        ptree_height P <= d ->
+            struct_valid P ->
+                forall (S : subst_ind),
+                    struct_valid (ptree_ug_l_inv P A S).
+Proof.
+induction d;
+intros P A LT PSV S.
+exfalso.
+destruct P;
+inversion LT.
+destruct P;
 unfold ptree_ug_l_inv;
-unfold ug_left_inv_batch, batch_sub;
 case nat_eqb eqn:EQ;
 try apply PSV;
+unfold ptree_height in *;
+fold ptree_height in *;
+apply le_S_n in LT;
 unfold ptree_ug_l_inv_fit;
 fold ptree_ug_l_inv_fit.
 
@@ -512,49 +631,30 @@ fold ptree_ug_l_inv_fit.
 
 all : subst.
 
-13 :  case (form_eqb phi AF) eqn:EQfn;
-      case b.
+13 :  case (form_eqb phi A) eqn:EQF.
+13 :  destruct b.
 
 2 : { rewrite ptree_ug_l_inv_fit_true.
       2 : apply EQ.
-      enough (struct_valid (loop_head (ptree_constraint P) (ug_left_inv_batch (ptree_left P) AF 0 S) (ptree_right P) (ptree_deg P) (ptree_ug_l_inv P AF S))) as PSV'.
+      enough (struct_valid (loop_head (ptree_constraint P) (ug_left_inv_batch (ptree_left P) A S) (ptree_right P) (ptree_deg P) (ptree_ug_l_inv P A S))) as PSV'.
       destruct P;
       try apply PSV';
       contradiction (PRec eq_refl).
       repeat split.
-      - apply (IHP _ PSV).
+      - apply (IHd _ _ LT PSV).
       - rewrite ptree_ug_l_inv_vars.
         apply PG_app.
       - apply PD_app.
-      - destruct (ptree_eq_dec (ptree_ug_l_inv P AF S) bot) as [EQ' | NE].
+      - destruct (ptree_eq_dec (ptree_ug_l_inv P A S) bot) as [EQ' | NE].
         apply (inl EQ').
         right.
         repeat split;
-        try rewrite P1G;
-        try rewrite P2G;
         try apply EQ;
-        try unfold ptree_left at 1 in EQ;
-        try rewrite bury_length, <- (@bury_unbury _ S n), bury_length in EQ;
-        try apply EQ;
-        repeat split;
         try rewrite ptree_ug_l_inv_constraint;
         try apply ptree_ug_l_inv_deg;
         try rewrite ptree_ug_l_inv_left;
-        try rewrite PG;
-        try rewrite P1G;
-        try rewrite P2G;
-        unfold flat_map;
-        fold (flat_map vars_in);
-        try rewrite ptree_ug_l_inv_vars;
-        try rewrite ug_l_formula_inv_vars;
-        unfold ug_left_inv_batch;
-        try rewrite batch_sub_false_head;
         try rewrite ptree_ug_l_inv_right;
-        try apply Order;
         try assumption;
-        try apply (IHP _ _ PSV);
-        try apply (IHP1 _ _ P1SV);
-        try apply (IHP2 _ _ P2SV);
         try reflexivity. }
 
 1 : { repeat split.
@@ -562,6 +662,84 @@ all : subst.
       apply PG_app.
       apply PD_app.
       apply (inl eq_refl). }
+
+19 : rewrite (ptree_ug_l_inv_fit_extra _ _ _ _ _ (PeanoNat.Nat.le_max_l _ _) (le_n _)), (ptree_ug_l_inv_fit_extra _ _ _ _ _ (PeanoNat.Nat.le_max_r _ _) (le_n _)).
+
+17 : rewrite (ptree_ug_l_inv_fit_extra _ _ _ _ _ (PeanoNat.Nat.le_max_l _ _) (le_n _)), (ptree_ug_l_inv_fit_extra _ _ _ _ _ (PeanoNat.Nat.le_max_r _ _) (le_n _)).
+
+1 : { rewrite (ptree_ug_l_inv_fit_extra _ _ _ _ _ (ptree_ug_l_inv_height _ _ _) (le_n _)).
+      rewrite !ptree_ug_l_inv_fit_true.
+      3 : rewrite !ptree_ug_l_inv_fit_true;
+          try rewrite (ptree_ug_l_inv_left _ _ PSV);
+          unfold ug_left_inv_batch;
+          try rewrite <- batch_sub_length;
+          try apply nat_eqb_eq.
+      all : try rewrite PG;
+            unfold length;
+            fold (@length formula) (@length bool);
+            try rewrite repeat_length;
+            try apply EQ.
+      repeat split.
+      1 : { refine (IHd _ _ (PeanoNat.Nat.le_trans _ _ _ _ LT) (IHd _ _ LT PSV _) _).
+            pose proof (ptree_ug_l_inv_height P (shift_substitution A (Datatypes.S v1) v2) (false :: b2 :: (repeat false (length S)))) as LT'.
+            rewrite !ptree_ug_l_inv_fit_true in LT'.
+            apply LT'.
+            rewrite PG.
+            unfold length in *;
+            fold (@length formula) (@length bool) in *.
+            rewrite repeat_length.
+            apply EQ. }
+      1 : rewrite ptree_ug_l_inv_vars;
+          unfold ug_left_inv_batch;
+          apply PG_app.
+      1 : apply PD_app.
+      all : try rewrite !ptree_ug_l_inv_left;
+            try rewrite !ptree_ug_l_inv_right;
+            try rewrite !ptree_ug_l_inv_constraint;
+            try rewrite !ptree_ug_l_inv_deg;
+            try reflexivity;
+            try apply PSV;
+            try apply (IHd _ _ LT PSV).
+      unfold ug_left_inv_batch.
+      unfold batch_sub at 1.
+      unfold ptree_left in EQ.
+      rewrite PG, <- batch_sub_length.
+      unfold batch_sub.
+      all : unfold length in *;
+            fold (@length bool) (@length formula) in *;
+            try rewrite repeat_length.
+      2 : apply (nat_eqb_eq _ _ EQ).
+      rewrite EQ.
+      unfold nat_eqb in EQ;
+      fold nat_eqb in EQ.
+      rewrite EQ.
+      unfold batch_sub_fit;
+      fold batch_sub_fit.
+      rewrite batch_sub_false.
+      unfold formula_sub, form_eqb;
+      fold form_eqb.
+      case (form_eqb (shift_substitution phi v1 v2) (univ (shift_substitution A (Datatypes.S v1) v2))) eqn:EQF.
+      destruct b2.
+      - assert (form_eqb (shift_substitution phi v1 v2) (shift_substitution (univ A) v1 v2) = true) as EQF'. apply EQF.
+        case form_eqb;
+        unfold ug_left_inv_formula, formula_sub.
+        admit.
+        admit.
+      - case form_eqb;
+        unfold ug_left_inv_formula;
+        rewrite formula_sub_false;
+        reflexivity.
+      - assert (form_eqb (shift_substitution phi v1 v2) (shift_substitution (univ A) v1 v2) = false) as EQF'. apply EQF.
+        case form_eqb;
+        unfold ug_left_inv_formula, formula_sub;
+        rewrite (shift_subst_neb_form_neb _ _ _ _ EQF');
+        reflexivity. }
+
+18 : assert ((ptree_height P1) <= d /\ (ptree_height P2) <= d) as [LT1 LT2].
+18 : split; lia.
+
+16 : assert ((ptree_height P1) <= d /\ (ptree_height P2) <= d) as [LT1 LT2].
+16 : split; lia.
 
 all : repeat rewrite ptree_ug_l_inv_fit_true;
       try rewrite PG;
@@ -586,9 +764,9 @@ all : repeat rewrite ptree_ug_l_inv_fit_true;
       try rewrite batch_sub_false_head;
       try rewrite ptree_ug_l_inv_right;
       try assumption;
-      try apply (IHP _ PSV);
-      try apply (IHP1 _ P1SV);
-      try apply (IHP2 _ P2SV);
+      try apply (IHd _ _ LT PSV);
+      try apply (IHd _ _ LT1 P1SV);
+      try apply (IHd _ _ LT2 P2SV);
       try reflexivity.
 
 all : try rewrite <- batch_sub_fit_true;
@@ -597,17 +775,4 @@ all : try rewrite <- batch_sub_fit_true;
       try rewrite batch_sub_fit_true;
       try reflexivity;
       try apply EQ.
-
-- unfold formula_sub, form_equiv;
-  fold form_equiv.
-  case (form_equiv phi (univ AF) 0) eqn:EQF.
-  destruct b2.
-  rewrite form_equiv_0_eq in EQF.
-  apply form_eqb_eq in EQF.
-  subst.
-  rewrite form_equiv_diff_shift_subst.
-
-all : pose proof (ug_l_inv_form_depth_le phi AF b2) as LE;
-      unfold ug_left_inv_formula;
-      lia.
-Qed.
+Admitted.
